\documentclass{article}
\usepackage{amsmath}
\usepackage{amsthm}
\usepackage{enumerate}
\usepackage[bookmarks=true]{hyperref}
\usepackage{bookmark}
\usepackage{graphicx}

\input{../../physics_common}
\title{Importance Sampling}
\author{Xie Xiaolei}
\date{\today}

\begin{document}
\maketitle
\section{Introduction}
We consider the model
\begin{eqnarray*}
V_n &=& A_n V_{n-1} \\
V_0 &=& x_0 \in \mathbb S^{d-1}\\
\end{eqnarray*}
Use the following notations
\begin{eqnarray*}
X_n &=& \frac{V_n}{\|V_n\|} \\
S_n &=& \log \|A_n \cdots A_1 x_0\| \\
\xi_n &=& S_n - S_{n-1} = \log\frac{\|A_n \cdots A_1 x_0\|}{\|A_{n-1}
  \cdots A_1 x_0\|} \\
&=& \log\left\| A_n \frac{A_{n-1} \cdots A_1 x_0}{\|A_{n-1} \cdots A_1
    x_0\|} \right\|\\
&=& \log \|A_n X_{n-1}\|
\end{eqnarray*}
The pair $(X_n, S_n)$ is a Markov additive process with transition
kernel $P$. Assume conditions (M) and (A) of Kesten \cite{Kesten1973}:
\begin{enumerate}
\item The top Lyapunov exponent is negative, i.e.
  \begin{equation}
    \label{eq:neg_top_Lyapunov}
    \inf_{n \geq 1} \E \log \|A_n \cdots A_1\| < 0    
  \end{equation}
\item $\exists \xi > 0$ such that $\lambda(\xi) = 1$, where
  $$
  \lambda(\xi) := \inf_{n \geq 1} (\E \|A_n \cdots A_1\|^\xi)^{1/n}
  $$
\item $\E[\|A\|^\xi \log^+\|A\|] < \infty$
\end{enumerate}

\section{Consistency}\label{sec:consistency}
By the law of large numbers
\begin{eqnarray*}
  && \P(|V| > u) \\
  &=& \lim_{n \to \infty} {1 \over n} \sum_{i=0}^n \1{|V_i| > u}
\end{eqnarray*}
Define
\[
R_n := \inf\{0 \leq i \leq n: V_i \in \mathcal C\}
\]
and
\[
K_i := \inf\{k \geq 1: k > K_{i-1}, V_k \in \mathcal C, K_0 = 0\}
\]
Then one can write
\begin{eqnarray*}
  && \lim_{n \to \infty} {1 \over n} \sum_{i=1}^n \1{|V_i| > u} \\
  &=& \lim_{n \to \infty} {1 \over n} \left[
    \sum_{i=0}^{K_{R_n}-1} \1{|V_i| > u} + \sum_{i=K_{R_n}}^n \1{|V_i| > u}
\right]
\end{eqnarray*}
For the 2nd term, by a Borel-Cantelli argument, it maybe shown
\[
\lim_{n \to \infty} {1 \over n}\sum_{i=K_{R_n}}^n \1{|V_i| > u} = 0
\]
For the 1st term,
\begin{eqnarray*}
&& \lim_{n \to \infty} {1 \over n} \sum_{i=0}^{K_{R_n}-1} \1{|V_i| >
  u}  \\
&=& \lim_{n \to \infty} {R_n \over n} {1 \over R_n} \sum_{i=1}^{R_n}
\sum_{j=K_{i-1}}^{K_i-1}\1{|V_i| > u} \\
&=& \pi(\mathcal C) \E_\gamma N_u
\end{eqnarray*}
where the law of large numbers of Markov chains has been used to reach
the last line. In addition, it is assumed
\begin{eqnarray*}
  V_{K_i} &\sim& \gamma \; \forall i \geq 0 \\
  \gamma(E) &=& \pi(E)/\pi(\mathcal C)\; \forall E \in \mathcal
  B(\mathcal C)
\end{eqnarray*}
Define
\begin{eqnarray*}
  T_u &=& \inf\{n \geq 1: |V_n| > u\} \\
  \tau &\overset{d}{=}& K_i - K_{i-1} \\
  N_u &:=& \sum_{i=0}^{\tau-1} \1{|V_i| > u}  \\
\end{eqnarray*}
Then $\E_\gamma N_u$ may be evaluated as
\begin{eqnarray*}
  && \E_\gamma N_u \\
  &=& \E_\gamma N_u \1{T_u < \tau} \\
  &=& \int_{\mathds S^{d-1}} \int_{\mathds R} \cdots \int_{\mathds
    S^{d-1}} \int_{\mathds R} N_u \1{T_u < \tau} \times \\
  && \prod_{i=1}^{T_u} e^{-\xi(s_i - s_{i-1}) + \lambda(\xi)}
  {r(x_{i-1}; \xi) \over r(x_{i}; \xi)}P_\xi(x_{i-1}, dx_i \times ds_i) \times \\
  && \prod_{i=T_u+1}^{\tau-1} P(x_{i-1}, dx_i \times d s_i) \\
  &=& \E_{\mathcal D} \left[
    N_u \1{T_u < \tau} e^{-\xi S_{T_u}} {r(x_0; \xi)
      \over r(x_{T_u}; \xi)}
  \right]
\end{eqnarray*}
where
\[
P_\xi(x_{i-1}, dx_i \times ds_i) = e^{\xi(s_i - s_{i-1}) -
  \lambda(\xi)} {r(x_i; \xi) \over r(x_{i-1}; \xi)} P(x_{i-1}, dx_i
\times ds_i)
\]
is the $\xi$-shifted transition kernel of the {\it Markov Additive
  process} $(X_n, S_n)$. $\xi$ is chosen such that 
\[
\lambda(\xi) = \lim_{n \to \infty} \log \left(
\E \|A_n \cdots A_1\|^\xi
\right)^{1/n} = 0
\]
$\E_{\mathcal D}$ denotes expectation taken with respect to the dual
measure defined as
\[
P_{\mathcal D} (x_i, dx_{i+1} \times ds) = \left\{
  \begin{array}{ll}
    P_\xi (x_i, dx_{i+1} \times ds) & \text{ if } i < T_u \\
    P(x_i, dx_{i+1} \times ds) & \text{ if } i \geq T_u \\
  \end{array}
\right.
\]
Because the top Lyapunov exponent is negative, it follows from a lemma
in Kesten \cite{Kesten1973} that there is a $s > 0$ such that
$\lambda(s) < 0$.

Thus we have obtained a consistent estimator
$\pi(\mathcal C)\mathcal E_u$ for $\P(|V| > u)$:
\begin{eqnarray*}
\P(|V| > u) &=& \pi(\mathcal C) \E_{\mathcal D} \mathcal E_u \\
&=& \pi(\mathcal C) \E_{\mathcal D} \left[
  N_u \1{T_u < \tau} e^{-\xi S_{T_u}} {r(x_0; \xi)
    \over r(x_{T_u}; \xi)}
\right]
\end{eqnarray*}

\section{Efficiency}\label{sec:efficiency}
\begin{lemma}
  Let $\beta \in \mathbb R$ satisfy
  \begin{enumerate}[(i)]
  \item
    \begin{equation}
      \label{eq:drift_cond1}
      \E \|A\|^\beta < \infty      
    \end{equation}
  \item 
    \begin{equation}
      \label{eq:drift_cond2}
    \inf_{\alpha > 0} {\E \|A\|^{\alpha + \beta}
      \over 
      \E \|A\|^{\beta}
    } < 1
    \end{equation}
  \end{enumerate}
  then $\forall \alpha > 0$ such that $\frac{\E\|A\|^{\beta +
      \alpha}}{\E\|A\|^\beta} < 1$ , we have
  \begin{equation}
    \label{eq:drift}
    \E_\beta \left[\left.
        |V_n|^\alpha r_\beta(|\tilde V_n|; \alpha) \I{C^\complement}(V_{n-1}) \right|
      \mathcal F_{n-1} \right] \leq |V_{n-1}|^\alpha r_\beta(|\tilde
    V_{n-1}|; \alpha) \I{C^\complement}(V_{n-1})
  \end{equation}
  where $r_\beta(\cdot; \alpha)$ is the unique right eigen function of the
  operator
  \[
  P_{\alpha, \beta} f(x) = \int |\hat a x|^\alpha f\left(
    {\hat a x \over |\hat a x|}
  \right) d\mu_A^\beta(\hat a)
  \]
  where the $\beta$-shifted measure $\mu_A^\beta$ satisfies
  \[
  d\mu_A^\beta(\hat a) = {\|\hat a\|^\beta d\mu_A(\hat a) \over \E\|A\|^\beta}
  \]
\end{lemma}

\begin{proof}
  Conditions \eqref{eq:drift_cond1} and \eqref{eq:drift_cond2} imply $\E_\beta
  \|A\|^\alpha < \infty$. Then, using the results of Buraczewski and
  Collamore et al \cite{BCDZ2014}, one may conclude that an eigen
  function $r_\beta(\cdot; \alpha)$ as well as an eigen measure
  $l_\beta(\cdot; \alpha)$ exists under the $\beta$-shifted
  measure. Thus, by defining the adjoint operator under  the shifted
  measure, the right eigen function $r_\beta(x; \alpha)$ can be represented as
  \[
  r_\beta(x; \alpha) = c \int_{S_+^{d-1}} \inn{x, y}^\alpha
  dl^*_{\beta}(x; \alpha)
  \]
Now, to prove \eqref{eq:drift}, consider
  \begin{eqnarray*}
    && \E_\beta \left[ |V_n|^\alpha r_\beta(\tilde V_n; \alpha) | \mathcal F_{n-1} \right]
    \\
    &=& \E_\beta\left[\int_{S_+^{d-1}} \inn{V_n, y}^\alpha dl^*_{\beta}(y; \alpha)|
      \mathcal F_{n-1} \right]
    \\
    &=& \E_\beta\left[\int_{S_+^{d-1}} (\inn{A_n V_{n-1}, y} + \inn{B_n,
        y})^\alpha dl^*_{\beta}(y; \alpha) | \mathcal F_{n-1} \right]
  \end{eqnarray*}
  \begin{enumerate}[(i)]
  \item if $\alpha < 1$, by subadditivity we have
    \begin{eqnarray*}
      &&\E_\beta\left[\int_{S_+^{d-1}} (\inn{A_n V_{n-1}, y} + \inn{B_n,
          y})^\alpha dl^*_{\beta}(y; \alpha) | \mathcal F_{n-1} \right]\\
      &\leq& \E_\beta\left[\int_{S_+^{d-1}} \inn{A_n V_{n-1}, y}^\alpha
        dl^*_{\beta}(y; \alpha) | \mathcal F_{n-1} \right]
      + \E_\beta\left[\int_{S_+^{d-1}} \inn{B_n, y}^\alpha dl^*_{\beta}(y; \alpha) |
        \mathcal F_{n-1} \right] \\
      &=& \E_\beta\left[|V_{n-1}|^\alpha |A_n \tilde V_{n-1}|^\alpha\int_{S_+^{d-1}}
        \inn{{A_n V_{n-1} \over |A_n V_{n-1}|}, y}^\alpha
        dl^*_{\beta}(y; \alpha) | \mathcal F_{n-1} \right] \\
      && + \E_\beta\left[\int_{S_+^{d-1}} \inn{B_n, y}^\alpha dl^*_{\beta}(y; \alpha) |
        \mathcal F_{n-1} \right] \\
      &=& |V_{n-1}|^\alpha \left\{
        (P_{\alpha, \beta} r_{\beta})(\tilde V_{n-1}; \alpha) +
        {1 \over |V_{n-1}|^\alpha} \E_\beta |B_n|^\alpha r_\beta(\tilde
        B_n; \alpha) \right\} \\
      &=& |V_{n-1}|^\alpha r_\beta(\tilde V_{n-1}; \alpha)\left\{
        \lambda_\beta(\alpha) +
        {1 \over |V_{n-1}|^\alpha r_\beta(\tilde V_{n-1}; \alpha)} \E_\beta
        |B_n|^\alpha r_\beta(\tilde B_n; \alpha) \right\} \\
    \end{eqnarray*}
    By assumption, $\E_\beta|B_n|^\alpha < \infty$; and
    $r_\beta(\tilde B_n; \alpha) < \infty$, $r_\beta(\tilde V_{n-1};
    \alpha) < \infty$ according to Buraczewski and Collamore \cite{BCDZ2014}.
    Hence the infimum of the expression in the curly bracket over all $n \geq 1$ is
    $\lambda_\beta(\alpha) < 1$. Therefore, when $|V_{n-1}|$ is
    sufficiently large, $\rho_{\beta}(\alpha)$ an be chosen such that
    \begin{eqnarray*}
      \rho_{\beta}(\alpha) &<& 1 \\
      \E_\beta \left[ |V_n|^\alpha r_\beta(\tilde V_n; \alpha)  \I{C^\complement}(V_{n-1})
        | \mathcal F_{n-1} \right] &\leq&
      \rho_\beta(\alpha) |V_{n-1}|^\alpha r_\beta(\tilde V_{n-1}; \alpha) \I{C^\complement}(V_{n-1})
    \end{eqnarray*}
    where $C^\complement$ denotes the complement of the set $C$:
    \[
    C = \left\{
      v: |v| \leq M, M = \left[
        \E_\beta (|B|^\alpha r_\beta(\tilde B; \alpha)) 
        \over
        [1 - \lambda(\alpha)] r_\beta(\tilde v; \alpha)
      \right]^{1/\alpha}
    \right\}
    \]
  \end{enumerate}    
% that there exist a unique
%   probability measure $l_\alpha$ on $\mathbb S_+^{d-1}$ and a unique
%   and strictly positive function $r_\alpha \in \mathscr C_b(\mathbb
%   S_+^{d-1})$ such that
%   \begin{eqnarray*}
%     P_\alpha r(x; \alpha) &=& \lambda(\alpha) r(x; \alpha) \\
%     l_\alpha P_\alpha (S) &=& \lambda(\alpha) l_\alpha(S) \\
%     \int_{S_+^{d-1}} r(x; \alpha) l_\alpha(dx) &=& 1
%   \end{eqnarray*}
\end{proof}
  Iterating \eqref{eq:drift} yields
  \[
  \E_\beta \left[
         |V_n|^\alpha r_\beta(|\tilde V_n|; \alpha) \prod_{i=1}^{n-1}\I{C^\complement}(V_i)\right]
      \leq \rho_\beta(\alpha)^{n-1} |V_1|^\alpha r_\beta(|\tilde V_1|; \alpha) \I{C^\complement}(V_1)
  \]
  Then it follows
  \[
  \E_\beta \left[
         |V_n|^\alpha r_\beta(|\tilde V_n|; \alpha) \prod_{i=1}^{n}\I{C^\complement}(V_i)\right]
      \leq \rho_\beta(\alpha)^{n-1} |V_1|^\alpha r_\beta(|\tilde V_1|; \alpha) \I{C^\complement}(V_1)
  \]
  But $\prod_{i=1}^{n}\I{C^\complement}(V_i)$ implies $\tau > n$, and in this
  case $|V_n| > M$, where
  \[
  M = \left[
        \E_\beta (|B|^\alpha r_\beta(\tilde B; \alpha)) 
        \over
        (1 - \lambda(\alpha)) r_\beta(\tilde v; \alpha)
      \right]^{1/\alpha}
  \]
  Hence
  \begin{eqnarray}
    \E_\beta \left[
      M^\alpha \inf_{|\tilde V_n|} r_\beta(|\tilde V_n|; \alpha) \1{\tau > n}\right]
    &\leq& \rho_\beta(\alpha)^{n-1} |V_1|^\alpha r_\beta(|\tilde V_1|; \alpha) \I{C^\complement}(V_1) \nonumber \\
    \P_\beta(\tau > n) &\leq& K \rho_\beta(\alpha)^{n-1} \label{eq:ret_time}
  \end{eqnarray}
  for some constant $K$.
  
%% \subsection{The Drift Condition}
%%% What follows is the proof in the 1D case.
% Consider
% \begin{eqnarray*}
%   && \int_E |y|^\alpha P_\beta(v, dy)  \\
%   &=& \int_E |A_n v + B_n|^\alpha \P_\beta\left(V_n \in [y, y +dy) |
%   V_{n-1} = v\right) \\
% &=& \int_{R^3} |A_n v + B_n|^\alpha d\mu_\beta(\log A_n, B_n, D_n) \\
% &=& \E_\beta |A_n v + B_n|^\alpha
% \end{eqnarray*}
% \begin{enumerate}[(i)]
% \item if $\alpha < 1$, $|\cdot|^\alpha$ is a concave and hence
%   subadditive function. We have
%   \begin{eqnarray*}
%     && \E_\beta |A_n v + B_n|^\alpha    \\
%     &\leq& |v|^{\alpha}\E_\beta|A_n|^\alpha + \E_\beta|B_n|^\alpha \\
%     &\leq& |v|^{\alpha}\left(
%       \E_\beta|A_n|^\alpha + |v|^{-\alpha}\E_\beta|B_n|^\alpha
%     \right)\\
%   \end{eqnarray*}
%   Clearly
%   \begin{eqnarray*}
%     \inf_{v} \left(
%       \E_\beta|A_n|^\alpha + |v|^{-\alpha}\E_\beta|B_n|^\alpha
%     \right) = \E_\beta|A_n|^\alpha
%   \end{eqnarray*}
%   Therefore, if there exists an $\alpha > 0$ such that
%   $\E_\beta|A_n|^\alpha < 1$, $|v|$ can be chosen sufficiently large
%   so that $\E_\beta|A_n|^\alpha + |v|^{-\alpha}\E_\beta|B_n|^\alpha <
%   1$. By definition,
%   \begin{eqnarray*}
%     && \E_\beta |A_n|^\alpha \\
%     &=& \int_{R^3} |A_n|^{\alpha + \beta} d\mu(\log A_n, B_n, D_n)
%     \times \\
%     && \left[
%       \int_{R^3} |A_n|^{\beta} d\mu(\log A_n, B_n, D_n)
%     \right]^{-1} \\
%     &=& {\E |A_n|^{\alpha + \beta} \over \E |A_n|^{\beta}}
%   \end{eqnarray*}
%   Since $\E|A_n|^{\zeta}$ is convex and by
%   assumption, $\E|A_n|^{\xi} =\E|A_n|^0= 1$, it immediately follows
% \[
% \exists s \in (0, \xi), \E |A_n|^s = \inf_{\zeta \in (0, \xi)} \E
% |A_n|^\zeta < 1
% \]
% Thus, for any given $\alpha \in (0, \xi)$, one can always find
% $\beta\in [0, \xi-\alpha]$ such that $\E_\beta |A_n|^\alpha = {\E
%   |A_n|^{\alpha + \beta} \over \E |A_n|^{\beta}} < 1$. Once $\beta$
% has been chosen accordingly, one can choose $v \notin (-M_\beta,
% M_\beta)$ so that $\E_\beta|A_n|^\alpha +
% |v|^{-\alpha}\E_\beta|B_n|^\alpha < 1$. Here
% \[
% M_\beta = \left({\E_\beta |B_n|^\alpha \over 1 - \E_\beta
%     |A_n|^\alpha}\right)^{1/\alpha}
% \]

% \item if $\alpha \geq 1$, by Minkowskii inequality,
%   \begin{eqnarray*}
%     && \E_\beta |A_n v + B_n|^\alpha \\
%     &\leq& |v|^\alpha\left[
%       (\E_\beta|A_n|^\alpha)^{1/\alpha} + {(\E_\beta
%         |A_n|^\alpha)^{1/\alpha} \over |v|}
%     \right]^\alpha
%   \end{eqnarray*}
%   The same arguments as in the $\alpha < 1$ case apply. But in this
%   case we have
%   \[
%   M_\beta = \left[{
%     (\E_\beta |B_n|^\alpha)^{1/\alpha}
%     \over
%     1 - (\E_\beta|A_n|^\alpha)^{1/\alpha}
%   }\right]^{1/\alpha}
% \]


% In this section we prove
% \[
% \E \left[ |V_n|^\alpha r_{\xi, \alpha}(\tilde V_n) | \mathcal F_{n-1} \right] \leq
% \rho |V_{n-1}|^\alpha r_{\xi,\alpha}(\tilde V_{n-1})
% \]
% for some $\rho < 1$.
% where 
% \begin{proof}
%   \begin{eqnarray*}
%     && \E \left[ |V_n|^\alpha r(\tilde V_n; \alpha) | \mathcal F_{n-1} \right]
%     \\
%     &=& \E\left[\int_{S_+^{d-1}} \inn{V_n, y}^\alpha dl^*_\alpha(y)|
%       \mathcal F_{n-1} \right]
%     \\
%     &=& \E\left[\int_{S_+^{d-1}} (\inn{A_n V_{n-1}, y} + \inn{B_n,
%         y})^\alpha dl^*_\alpha(y) | \mathcal F_{n-1} \right]
%   \end{eqnarray*}
%   \begin{enumerate}[(i)]
%   \item if $\alpha < 1$, by subadditivity we have
%     \begin{eqnarray*}
%       &&\E\left[\int_{S_+^{d-1}} (\inn{A_n V_{n-1}, y} + \inn{B_n,
%           y})^\alpha dl^*_\alpha(y) | \mathcal F_{n-1} \right]\\
%       &\leq& \E\left[\int_{S_+^{d-1}} \inn{A_n V_{n-1}, y}^\alpha
%         dl^*_\alpha(y) | \mathcal F_{n-1} \right]
%       + \E\left[\int_{S_+^{d-1}} \inn{B_n, y}^\alpha dl^*_\alpha(y) |
%         \mathcal F_{n-1} \right] \\
%       &=& \E\left[|V_{n-1}|^\alpha |A_n \tilde V_{n-1}|^\alpha\int_{S_+^{d-1}}
%         \inn{{A_n V_{n-1} \over |A_n V_{n-1}|}, y}^\alpha
%         dl^*_\alpha(y) | \mathcal F_{n-1} \right] \\
%       && + \E\left[\int_{S_+^{d-1}} \inn{B_n, y}^\alpha dl^*_\alpha(y) |
%         \mathcal F_{n-1} \right] \\
%       &=& |V_{n-1}|^\alpha \left\{
%         (P_\alpha r_\alpha)(\tilde V_{n-1}) +
%         {1 \over |V_{n-1}|^\alpha} \E |B_n|^\alpha r(\tilde
%         B_n; \alpha) \right\} \\
%       &=& |V_{n-1}|^\alpha r(\tilde V_{n-1}; \alpha)\left\{
%         \lambda(\alpha) +
%         {1 \over |V_{n-1}|^\alpha r(\tilde V_{n-1}; \alpha)} \E
%         |B_n|^\alpha r(\tilde B_n; \alpha) \right\} \\
%     \end{eqnarray*}
%     Clearly $\E\left[|B_n|^\alpha r(\tilde B_n; \alpha)\right] <
%     \infty$. Hence the infimum of the expression in the curly bracket
%     over all $n \geq 1$ is $\lambda(\alpha) < 1$. Therefore, when
%     $|V_{n-1}|$ is sufficiently large, we have
%     \[
%     \E \left[ |V_n|^\alpha r(\tilde V_n; \alpha) | \mathcal F_{n-1} \right] \leq
%     \rho |V_{n-1}|^\alpha r(\tilde V_{n-1}; \alpha)
%     \]
%   \end{enumerate}    
% \end{proof}

\begin{theorem}
  The estimator $\mathcal E_u$ has bounded relative error, i.e.
  \begin{equation*}
    \limsup_{u \to \infty} {\var(\mathcal E_u) \over [\P(|V| > u)]^2} < \infty
  \end{equation*}
\end{theorem}
\begin{proof}
  The claim is equivalent to
  \[
  \limsup_{u \to \infty} {\E_D \mathcal E_u^2 \over [\P(|V| > u)]^2} < \infty
  \]
  By Kesten's theorem \cite{Kesten1973}, $\P(|V| > u) \sim C
  u^{-\xi}$. Hence, to prove the claim, one needs to check
  $u^{2\xi}\E_D \mathcal E_u^2 < \infty$, i.e.
  \[
  f(\xi) = \limsup_{u \to \infty} \E_D  \left[u^{2\xi}
    N_u^2 \1{T_u < \tau} e^{-2\xi S_{T_u}} {r^2(x_0; \xi)
      \over r^2(x_{T_u}; \xi)}\right]
  < \infty
  \]
  In the rest of the proof, we write $c$ for any constant whose value
  is of no importance.
  \begin{enumerate}[(i)]
  \item We first consider the case $\log \E \|A\|^{-(\xi + \epsilon)}
    < -\inf_{\alpha \in \mathbb R} \log \E \|A\|^\alpha$ for some
    $\epsilon > 0$. Using the fact $|V_{T_u} > u|$  we obtain
  \begin{eqnarray*}
    f(\xi) &\leq& \limsup_{u \to \infty} \E_D \left[
                  N_u^2  \left|
                  \frac{
                  \sum_{n=0}^{T_u} A_{T_u} \cdots A_{n+1} B_n 
                  }{
                  |A_{T_u} \cdots A_1 V_0|
                  }
                  \right|^{2 \xi}
                  \frac{
                  r(X_0; \xi)^2
                  }{
                  r(X_{T_u}; \xi)^2
                  } \1{T_u < \tau}
    \right] \\
  \end{eqnarray*}
  where $1/r + 1/s = 1$. Then H\"older's inequality gives
  \begin{eqnarray*}
    f(\xi) &\leq& \limsup_{u \to \infty} (\E_D N_u^{2r})^{1/r}
                  \left(\E_D \left|
                  \frac{
                  \sum_{n=0}^{T_u} A_{T_u} \cdots A_{n+1} B_n 
                  }{
                  |A_{T_u} \cdots A_1 V_0|
                  }
                  \right|^{2 s \xi} \1{T_u < \tau}
                  \right)^{1/s} \\
           &\leq& c \limsup_{u \to \infty} f_1(u) f_2(u, \xi)
  \end{eqnarray*}
  For $f_2(u,\xi)$ Minkowski's inequality yields
  \begin{eqnarray*}
    f_2(u, \xi)^{1/2\xi} &\leq& \sum_{n=0}^\infty \left(\E_D \left[
                                \frac{
                                |A_{T_u} \cdots A_{n+1} B_n |^{2s\xi}
                                }{
                                |A_{T_u} \cdots A_1 V_0|^{2s\xi}
                                } \1{n \leq T_u < \tau}
                                \right]\right)^{1/2s\xi} \\
                         &=& \sum_{n=0}^\infty \left(\E \left[
                             \frac{
                             |A_{T_u} \cdots A_{n+1} B_n |^{2s\xi}
                             }{
                             |A_{T_u} \cdots A_1 X_0|^{\xi(2s - 1)}
                             }
                             \frac{
                             r_{\xi}(X_{T_u})
                             }{
                             r_{\xi}(X_{0})
                             }
                             {1 \over |V_0|^{2s\xi}}\1{n \leq T_u < \tau}
                             \right]\right)^{1/2s\xi} \\
                         &\leq& c \sum_{n=0}^\infty
                                \left(\E_{-\xi(2s - 1)} \left[
                                |A_{T_u} \cdots A_{n+1} B_n |^{2s\xi}
                                \lambda(-\xi(2s - 1))^{T_u}
                                \1{n \leq T_u < \tau}
                                \right]\right)^{1/2s\xi} \\
                         &=& c \sum_{n=0}^\infty [\E_{-\xi(2s - 1)}
                             f_{2,n}(u,\xi)]^{1/2s\xi}
  \end{eqnarray*}
  As for $\E_{-\xi(2s - 1)} f_{2,n}(u,\xi)$ we have
  \begin{eqnarray*}
    && \E_{-\xi(2s - 1)} f_{2,n}(u,\xi) \\
    &\leq& \sum_{k=n}^\infty \E_{-\xi(2s - 1)}\left(
           \|A_k \cdots A_{n+1}\|^{2s\xi}|T_u = k \right)
           \E_{-\xi(2s - 1)} |B_n|^{2s\xi} \times \\
    && \lambda(-\xi(2s - 1))^{k} \1{\tau > k}
       \P_{-\xi(2s - 1)}(T_u \geq k)
  \end{eqnarray*}
  Obviously $\1{\tau > T_u} \P_{-\xi(2s - 1)}(T_u \geq k) \leq
  \P_{-\xi(2s - 1)}(\tau > k-1)$, and by assumption $\E_{-\xi(2s - 1)}
  |B_n|^{2s\xi} < \infty$. We also note
  \[
  \lim_{k \to \infty}
  \left[ \E_{-\xi(2s - 1)}\left(
    \|A_k \cdots A_{n+1}\|^{2s\xi}|T_u = k
  \right) \right]^{1/(k-n)} = \lambda_{-\xi(2s - 1)}(2s\xi)
  \]
  and
  \[
  \inf_{k \geq n+1}
  \left(
    \E_{-\xi(2s - 1)}\|A_k \cdots A_{n+1}\|^{2s\xi}
  \right)^{1/(k - n)} = \lambda_{-\xi(2s - 1)}(2s\xi)
  \]
  Hence for any $a > 1$, $\exists N \geq 1$ such that $\forall k
  \geq n + N$, $(\E_{-\xi(2s - 1)}\|A_{n+N} \cdots
  A_{n+1}\|^{2s\xi})^{1/N} < a \lambda_{-\xi(2s -
    1)}(2s\xi)$. Thus we have
  \begin{eqnarray*}
    && \E_{-\xi(2s - 1)} f_{2,n}(u,\xi) \\
    &\leq& c_1 + c_2 \sum_{k=n+N}^\infty \left[
           a \lambda_{-\xi(2s + 1)}(2s\xi)
           \right]^{k-n} \lambda[-\xi(2s - 1)]^{k}
           \P_{-\xi(2s - 1)}(\tau > k-1)
  \end{eqnarray*}
  
  where $\lambda_{-\xi(2s - 1)}(\alpha) < 1$.

  
    By Minkowski's inequality,
    \begin{eqnarray*}
      && [\E |f_u(\xi)|]^{1/\xi} \\
      &\leq& \sum_{n=1}^{\infty} \left[\E \left(
          N_u^2 \frac{
            |A_{T_u} \cdots A_{n+1} \tilde B_n|^{\xi}
          }{
            |A_{T_u} \cdots A_{1} \tilde V_0|^{\xi}
          } \frac{
            |B_n|^{\xi}
          }{
            |V_0|^{\xi}
          } \frac{
            r(X_0; \xi)
          }{
            r(X_{T_u}; \xi)
          }
          \1{n \leq T_u < \tau}
      \right)\right]^{1/\xi} \\
    &\leq& \sum_{n=1}^{\infty} \left[ \E f_{u,n}(\xi) \right]^{1/\xi}
    \end{eqnarray*}
    Applying H\"older's inequality leads to
    \begin{eqnarray*}
      \E f_{u,n}(\xi) &\leq& (\E N_u^{2r})^{1/r} \left(
        \E \frac{
          |A_{T_u} \cdots A_{n+1} \tilde B_n|^{s \xi}
        }{
          |A_{T_u} \cdots A_{1} \tilde V_0|^{s \xi}
        } \right)^{1/s} \times \\
      &&
      \left[
        \E \frac{
          |B_n|^{t\xi} r^t_\xi(X_0)
        }{
          |V_0|^{t\xi} r^t_\xi(X_{T_u})
        } \right]^{1/t}
      [\P(n \leq T_u < \tau)]^{1/s}
    \end{eqnarray*}
    where $1/r + 2/s + 1/t = 1$. First note
    \begin{eqnarray*}
      && \E \frac{
        |A_{T_u} \cdots A_{n+1} \tilde B_n|^{s \xi}
      }{
        |A_{T_u} \cdots A_{1} \tilde V_0|^{s \xi}
      } \\
      &\leq& \E \left\{\E_{-s\xi} \left[\left.
            \|A_{T_u} \cdots A_{n+1} \|^{s \xi} \frac{
              r(X_0; -s\xi)
            }{
              r(X_{T_u}; -s\xi)
            } \lambda(-s\xi)^{T_u} \right| T_u\right] \right\}
    \end{eqnarray*}
    Here the existance of the eigenvalue $\lambda(-s\xi)$ is ensured
    by the assumption $\E \|A\|^{-(\xi + \epsilon)} < \infty$. On this
    condition, one can always choose $s > 1$ such that $s \xi < \xi +
    \epsilon$ and hence $\E \|A\|^{-s\xi} < \infty$. Because
    $r(\cdot; -s\xi)$ is bounded from above and below, we may write
    \begin{eqnarray*}
      && \E \left\{\E_{-s\xi} \left[\left.
            \|A_{T_u} \cdots A_{n+1} \|^{s \xi} \frac{
              r(X_0; -s\xi)
            }{
              r(X_{T_u}; -s\xi)
            } \lambda(-s\xi)^{T_u} \right| T_u\right] \right\} \\
      &\leq& c \E \left\{ \lambda(-s\xi)^{T_u} \E_{-s\xi} \left[\left.
            \|A_{T_u} \cdots A_{n+1} \|^{s \xi} \right| T_u\right]
      \right\} \\
      &\leq& c \E \left\{ \lambda(-s\xi)^{T_u} (\E_{-s\xi} \|A\|^{s
          \xi})^{T_u - n}\right\} \\
      &=& c \lambda(-s\xi)^n
    \end{eqnarray*}
    where $c$ is some constant. As for $\E N_u^{2r}$, we have
    \begin{eqnarray*}
      \E N_u^{2r} &\leq& \E \tau^{2r} \\
      &\leq& \sum_{i=1}^\infty i^{2r} \P(\tau > i -1) \\
      &\leq& 1 + \sum_{i=2}^\infty i^{2r} K \rho(\alpha)^{i-2} < \infty
    \end{eqnarray*}
    for some $0 < \alpha < \xi$. In the last step, we have used
    \eqref{eq:ret_time}. As regard $\P(n \leq T_u < \tau)$, we have
    \begin{eqnarray*}
      && \P(n \leq T_u < \tau) \\
      &\leq& \P(n < \tau) \\
      &\leq& K \rho(\alpha)^{n-1}
    \end{eqnarray*}
    So we may write
    \[
    \E f_{u, n}(\xi) \leq c \lambda(-s\xi)^{n/s} \rho(\alpha)^{(n-1)/s}
    \]
    Because $\rho(\alpha)$ can be chosen arbitrarily close but greater
    than $\lambda(\alpha) < 1$, the assumption $\inf_{\alpha \in
      \mathbb R} \log \lambda(\alpha) < -\log \lambda_{-(\xi+\epsilon)}$ implies
    $\alpha$ and $s$ can be chosen such that $\rho(\alpha) <
    1/\lambda(-s\xi)$. Then it follows
    \begin{eqnarray*}
      \sum_{n=1}^{\infty} [\E f_{u,n}(\xi)]^{1/\xi}  &\leq&
      c \rho_{\alpha}^{-1/s\xi}\sum_{n=1}^{\infty}
      \left[\rho(\alpha)\lambda(-s\xi)\right]^{n/s\xi} < \infty
    \end{eqnarray*}
    \item 
  \end{enumerate}
\end{proof}


\bibliographystyle{unsrt}
\bibliography{../../thesis/econophysics}
\end{document}
